ifc/ifc_sig.v
@@ -17,6 +17,8 @@ Require Import floyd.reptype_lemmas.
 Require Import floyd.field_at.
 Require Import floyd.client_lemmas.
 Require Export ifc.clsf_expr.
+Require Import floyd.nested_field_lemmas.
+Require Import floyd.proj_reptype_lemmas.
 Require Import List. Import ListNotations.
 
 Local Open Scope logic.
@@ -267,6 +269,45 @@ Axiom ifc_set: forall Delta id P Q R (N: T -> stack_clsf) (A: T -> heap_clsf) (e
     (fun x => (normal_ret_assert (PROPx (P x) 
            (LOCALx (temp id (v x) :: remove_localdef_temp id (Q x)) (SEPx (R x))))))
     (normalPostClsf (fun x i => if Pos.eqb i id then l2 x else N x i))
+    (normalPostClsf A).
+
+Axiom ifc_load: forall Delta P Q R (N: T -> stack_clsf) (A: T -> heap_clsf) sh n id e
+  (t t_root: type) (gfs0 gfs1 gfs: T -> list gfield) (l1 l2: T -> label)
+  (p q: T -> val) (v : T -> val)
+  (* dependent types FTW: *)
+  (v' : forall (x: T), reptype (nested_field_type t_root (gfs0 x))),
+  (* VST preconditions: *)
+  typeof_temp Delta id = Some t ->
+  is_neutral_cast (typeof e) t = true ->
+  type_is_volatile (typeof e) = false ->
+  (forall x, ENTAIL Delta, PROPx (P x) (LOCALx (Q x) (SEPx (R x))) |--
+     local (`(eq (q x)) (eval_lvalue e))) ->
+  (forall x, ENTAIL Delta, PROPx (P x) (LOCALx (Q x) (SEPx (R x))) |--
+     !! ((q x) = field_address t_root (gfs x) (p x))) ->
+  (forall x, typeof e = nested_field_type t_root (gfs x)) ->
+  (forall x, (gfs x) = (gfs1 x) ++ (gfs0 x)) ->
+  (forall x, nth_error (R x) n = Some (field_at sh t_root (gfs0 x) (v' x) (p x))) ->
+  readable_share sh ->
+  (forall x, JMeq (proj_reptype (nested_field_type t_root (gfs0 x)) (gfs1 x) (v' x)) (v x)) ->
+  (forall x, ENTAIL Delta, PROPx (P x) (LOCALx (Q x) (SEPx (R x))) |--
+    (tc_lvalue Delta e) &&
+    local `(tc_val (typeof e) (v x))) ->
+  (forall x, ENTAIL Delta, PROPx (P x) (LOCALx (Q x) (SEPx (R x))) |--
+    (!! legal_nested_field t_root (gfs x))) ->
+  (* IFC preconditions: *)
+  (forall x, ENTAIL Delta, PROPx (P x) (LOCALx (Q x) (SEPx (R x))) |--
+                 !! (clsf_lvalue (N x) e = Some (l1 x) /\
+                    (forall bl ofs, (q x) = Vptr bl ofs -> A x (bl, ofs) = (l2 x)))) ->
+  ifc_def T Delta
+    (fun x => (|>PROPx (P x) (LOCALx (Q x) (SEPx (R x)))))
+    N
+    A
+    (Sset id e)
+    (fun x => (normal_ret_assert (PROPx (P x) 
+                                 (LOCALx (temp id (v x) :: remove_localdef_temp id (Q x))
+                                 (SEPx (R x))))))
+    (normalPostClsf (fun x id0 =>
+           if Pos.eqb id0 id then lub (l1 x) (l2 x) else N x id0))
     (normalPostClsf A).
 
 Axiom ifc_store:
